
      ---------------------------------------------------
        An equivalent inductive-inductive definition of
                      ordinal notations
      ---------------------------------------------------

            Fredrik Nordvall Forsberg, April 2019


The metatheory of inductive-recursive definitions (A, f), where the
recursive function f : A â†’ A is an endofunction on the inductively
defined type A (e.g. (ğ’ª, fst) here) is in general not well explored.
However, in this case fst is only used strictly positively in ğ’ª and <,
which means that its graph can be defined inductive-inductively, and
in turn used instead of the recursively defined fst.  This reduces the
inductive-inductive-recursive construction to an inductive-inductive
one, which is known to be sound.

\begin{code}

module OrdinalNotationsWithoutRecursion where

open import Agda.Builtin.Equality
open import Data.Empty.Irrelevant
open import Relation.Nullary using (Â¬_)
open import Relation.Binary.PropositionalEquality using (_â‰¢_; congâ‚‚)
open import Data.Sum using (injâ‚; injâ‚‚) renaming (_âŠ_ to _âˆ¨_)
open import Data.Product -- using (Î£; Î£-syntax; _Ã—_)

open import OrdinalNotations

infix 30 _<'_
infix 30 _â‰¥'fst_

mutual

 data ğ’ª' : Set where
  ğŸ : ğ’ª'
  Ï‰^_+_[_] : (a b : ğ’ª') â†’ .(a â‰¥'fst b) â†’ ğ’ª'

 data _<'_ : ğ’ª' â†’ ğ’ª' â†’ Set where
  <â‚ : {a : ğ’ª'}
     â†’ a â‰¢ ğŸ â†’ ğŸ <' a
  <â‚‚ : {a b c d : ğ’ª'} .{r : a â‰¥'fst c} .{s : b â‰¥'fst d}
     â†’ a <' b â†’ Ï‰^ a + c [ r ] <' Ï‰^ b + d [ s ]
  <â‚ƒ : {a b c : ğ’ª'} .{r : a â‰¥'fst b} .{s : a â‰¥'fst c}
     â†’ b <' c â†’ Ï‰^ a + b [ r ] <' Ï‰^ a + c [ s ]

 data _â‰¡fst_ : ğ’ª' â†’ ğ’ª' â†’ Set where
   ğŸâ‰¡ğŸ : ğŸ â‰¡fst ğŸ
   bâ‰¡fst[Ï‰^b+[â€¦]] : {b d : ğ’ª'} .{s : b â‰¥'fst d} -> b â‰¡fst (Ï‰^ b + d [ s ])

 _fst<'_ : ğ’ª' â†’ ğ’ª' â†’ Set
 a fst<' b = Î£[ c âˆˆ ğ’ª' ] ((c â‰¡fst a) Ã— c <' b)

 _â‰¥'fst_ : ğ’ª' â†’ ğ’ª' â†’ Set
 a â‰¥'fst b = b fst<' a âˆ¨ a â‰¡fst b

fst' : ğ’ª' â†’ ğ’ª'
fst'  ğŸ               = ğŸ
fst' (Ï‰^ a + _ [ _ ]) = a

sound-â‰¡fst : (a b : ğ’ª') -> a â‰¡fst b -> a â‰¡ fst' b
sound-â‰¡fst .ğŸ ğŸ                ğŸâ‰¡ğŸ            = refl
sound-â‰¡fst a .(Ï‰^ a + _ [ _ ]) bâ‰¡fst[Ï‰^b+[â€¦]] = refl

complete-â‰¡fst : (a b : ğ’ª') -> a â‰¡ fst' b -> a â‰¡fst b
complete-â‰¡fst .ğŸ ğŸ                refl = ğŸâ‰¡ğŸ
complete-â‰¡fst .b (Ï‰^ b + c [ r ]) refl = bâ‰¡fst[Ï‰^b+[â€¦]]

sound-fst<' : (a b : ğ’ª') -> a fst<' b -> fst' a <' b
sound-fst<' .ğŸ                b (.ğŸ , ğŸâ‰¡ğŸ , q)            = q
sound-fst<' .(Ï‰^ d + _ [ _ ]) b (d , bâ‰¡fst[Ï‰^b+[â€¦]] , q) = q

complete-fst<' : (a b : ğ’ª') -> fst' a <' b -> a fst<' b
complete-fst<' ğŸ                b p = ğŸ , ğŸâ‰¡ğŸ , p
complete-fst<' (Ï‰^ a + c [ r ]) b p = a , bâ‰¡fst[Ï‰^b+[â€¦]] , p

\end{code}

We can prove that ğ’ª defined simultaneously with fst is isomorphic to
ğ’ª' defined simultaneously with the graph of fst.

\begin{code}

mutual

  to : ğ’ª -> ğ’ª'
  to ğŸ                = ğŸ
  to (Ï‰^ a + b [ r ]) = Ï‰^ (to a) + (to b) [ to-â‰¥ r ]

  to-< : {a b : ğ’ª} -> a < b -> (to a) <' (to b)
  to-< {b = ğŸ}              (<â‚ p) = âŠ¥-elim (p refl)
  to-< {b = Ï‰^ a + c [ r ]} (<â‚ p) = <â‚ (Î» ())
  to-<                      (<â‚‚ p) = <â‚‚ (to-< p)
  to-<                      (<â‚ƒ p) = <â‚ƒ (to-< p)

  to-â‰¥ : {a b : ğ’ª} -> a â‰¥ fst b -> (to a) â‰¥'fst (to b)
  to-â‰¥ {b = ğŸ}              (injâ‚ p) = injâ‚ (_ , ğŸâ‰¡ğŸ , to-< p)
  to-â‰¥ {b = Ï‰^ b + c [ r ]} (injâ‚ p) = injâ‚ (_ , bâ‰¡fst[Ï‰^b+[â€¦]] , to-< p)
  to-â‰¥ {b = ğŸ}              (injâ‚‚ refl) = injâ‚‚ ğŸâ‰¡ğŸ
  to-â‰¥ {b = Ï‰^ b + c [ r ]} (injâ‚‚ refl) = injâ‚‚ bâ‰¡fst[Ï‰^b+[â€¦]]

mutual

  from : ğ’ª' -> ğ’ª
  from ğŸ                = ğŸ
  from (Ï‰^ a + b [ r ]) = Ï‰^ (from a) + (from b) [ from-â‰¥ r ]

  from-< : {a b : ğ’ª'} -> a <' b -> (from a) < (from b)
  from-< {b = ğŸ}              (<â‚ p) = âŠ¥-elim (p refl)
  from-< {b = Ï‰^ b + c [ r ]} (<â‚ p) = <â‚ (Î» ())
  from-<                      (<â‚‚ p) = <â‚‚ (from-< p)
  from-<                      (<â‚ƒ p) = <â‚ƒ (from-< p)

  from-â‰¥ : {a b : ğ’ª'} -> a â‰¥'fst b -> (from a) â‰¥ fst (from b)
  from-â‰¥ {b = ğŸ}              (injâ‚ (ğŸ , ğŸâ‰¡ğŸ , p))             = injâ‚ (from-< p)
  from-â‰¥ {b = Ï‰^ b + c [ r ]} (injâ‚ (.b , bâ‰¡fst[Ï‰^b+[â€¦]] , p)) = injâ‚ (from-< p)
  from-â‰¥                      (injâ‚‚ ğŸâ‰¡ğŸ)                       = injâ‚‚ refl
  from-â‰¥ (injâ‚‚ bâ‰¡fst[Ï‰^b+[â€¦]])                                 = injâ‚‚ refl

-- An isomorphism is especially easy to establish, because of the
-- irrelevant equations

Ï‰'^_+_[_]-equal : âˆ€ {a b a' b'} .{r r'} â†’ (a â‰¡ a') â†’ (b â‰¡ b') â†’
                  (ğ’ª'.Ï‰^ a + b [ r ]) â‰¡ (Ï‰^ a' + b' [ r' ])
Ï‰'^_+_[_]-equal refl refl = refl

Ï‰^_+_[_]-equal : âˆ€ {a b a' b'} .{r r'} â†’ (a â‰¡ a') â†’ (b â‰¡ b') â†’
                 (ğ’ª.Ï‰^ a + b [ r ]) â‰¡ (Ï‰^ a' + b' [ r' ])
Ï‰^_+_[_]-equal refl refl = refl


to-from : (a : ğ’ª') -> to (from a) â‰¡ a
to-from ğŸ                = refl
to-from (Ï‰^ a + b [ r ]) = Ï‰'^_+_[_]-equal (to-from a) (to-from b)

from-to : (b : ğ’ª) -> from (to b) â‰¡ b
from-to ğŸ                = refl
from-to (Ï‰^ a + b [ r ]) = Ï‰^_+_[_]-equal (from-to a) (from-to b)

\end{code}
